testdata/export/frame_share_parent.cue
@@ -1,0 +1,2 @@
+a: {outer: 1, inner: {r: outer}}
+b: {outer: 2, inner: {r: outer}}
